providers/test/Test.Hash.fst
@@ -8,16 +8,17 @@ module M = LowStar.Modifies
 module MP = LowStar.ModifiesPat
 
 open LowStar.BufferOps
+open Spec.Hash.Helpers
 
 open ST
 
 let main (): St unit =
-  let s1 = H.create H.SHA256 in
+  let s1 = H.create SHA2_256 in
   let h1 = ST.get () in
-  let s2 = H.create H.SHA384 in
+  let s2 = H.create SHA2_384 in
   let h2 = ST.get () in
   H.frame_invariant M.loc_none s1 h1 h2;
-  H.init #(Ghost.hide H.SHA256) s1;
+  H.init #(Ghost.hide SHA2_256) s1;
   let h3 = ST.get () in
   H.frame_invariant (H.footprint s1 h1) s2 h2 h3;
-  H.init #(Ghost.hide H.SHA384) s2
+  H.init #(Ghost.hide SHA2_384) s2
